src/Maps.v
@@ -1,31 +1,29 @@
 From CoreErlang Require Export Equalities.
 Import ListNotations.
 
-Section map_builders.
-
 (** Building Val maps based on the Val ordering Val_less *)
-Fixpoint map_insert (k v : Val) (kl : list Val) (vl : list Val) : (list Val) * (list Val) :=
-match kl, vl with
-| [], [] => ([k], [v])
-| k'::ks, v'::vs => if Val_ltb k k' 
-                    then (k::k'::ks, v::v'::vs) 
-                    else
-                       if Val_eqb k k' 
-                       then (k'::ks, v'::vs) 
-                       else (k'::(fst (map_insert k v ks vs)), v'::(snd (map_insert k v ks vs)))
-| _, _ => ([], [])
+Fixpoint map_insert (k v : Val) (m : list (Val * Val))
+  : (list (Val * Val)) :=
+match m with
+| [] => [(k,v)]
+| (k',v')::ms => if Val_ltb k k' 
+                 then ((k, v)::(k',v')::ms) 
+                 else
+                    if Val_eqb k k' 
+                    then m
+                    else (k', v')::(map_insert k v ms)
 end.
 
 (** Create maps without duplicates based on the ordering *)
-Fixpoint make_val_map (kl vl : list Val) : (list Val) * (list Val) :=
-match kl, vl with
-| [], [] => ([], [])
-| k::ks, v::vs => map_insert k v (fst (make_val_map ks vs)) (snd (make_val_map ks vs))
-| _, _ => ([], [])
+Fixpoint make_val_map (l: list (Val * Val)) : list (Val * Val) :=
+match l with
+| [] => []
+| (k,v)::vs => map_insert k v (make_val_map vs)
 end.
 
-(* Compute make_val_map [VLit (Integer 5); VLit (Integer 5); VLit (Atom ""%string)] 
-                       [VLit (Integer 5); VLit (Integer 7); VLit (Atom ""%string)]. *)
+Goal make_val_map [(VLit 1%Z, VLit 1%Z);(VLit 1%Z, VLit 2%Z)] =
+    [(VLit 1%Z, VLit 2%Z)].
+Proof. simpl. reflexivity. Qed.
 
 Fixpoint flatten_list {A : Type} (l : list (A * A)) : list A :=
 match l with
@@ -67,154 +65,3 @@ Proof.
     destruct l. inversion H. destruct l. inversion H.
     simpl length in H. simpl. rewrite IHn; [reflexivity|nia].
 Qed.
-
-Fixpoint make_map_vals (l l' : list Val) : list Val  :=
-match l, l' with
-| [], [] => []
-| k::ks, v::vs => k::v::(make_map_vals ks vs)
-| k::ks, _ => [k]
-| _, _ => []
-end.
-
-Lemma length_make_map_vals l : forall l',
-  length l = length l' ->
-  length (make_map_vals l l') = length l * 2.
-Proof.
-  induction l; intros.
-  * apply eq_sym, length_zero_iff_nil in H. subst. auto.
-  * simpl in *. destruct l'.
-    - simpl in H. congruence.
-    - inversion H. simpl. rewrite (IHl l' H1). lia.
-Qed.
-
-Lemma length_make_map_vals2 l : forall l',
-  length l = S (length l') ->
-  length (make_map_vals l l') = length l' * 2 + 1.
-Proof.
-  induction l; intros.
-  * inversion H.
-  * simpl in *. destruct l'.
-    - simpl in H. apply Nat.succ_inj in H. apply length_zero_iff_nil in H.
-      subst. simpl. auto.
-    - inversion H. simpl. rewrite (IHl l' H1). lia.
-Qed.
-
-Lemma make_map_vals_eq kvals : forall kvals0 vvals vvals0,
-  length kvals = length vvals ->
-  length kvals0 = length vvals0 ->
-  length kvals = length kvals0 ->
-  make_map_vals kvals vvals = make_map_vals kvals0 vvals0
-->
-  kvals = kvals0 /\ vvals = vvals0.
-Proof.
-  induction kvals; intros.
-  * apply eq_sym, length_zero_iff_nil in H. apply eq_sym, length_zero_iff_nil in H1. subst.
-    apply eq_sym, length_zero_iff_nil in H0. subst.
-    auto.
-  * pose (element_exist _ _ H).
-    pose (element_exist _ _ H1). inversion e. inversion e0.
-    destruct H3, H4. subst. clear e. clear e0.
-    pose (element_exist _ _ H0). inversion e. destruct H3. clear e.
-    subst. simpl in H2. inversion H2. subst.
-    inversion H. inversion H0. inversion H1.
-    pose (IHkvals _ _ _ H4 H5 H7 H6). destruct a. subst. auto.
-Qed.
-
-Lemma make_map_vals_eq_rev kvals kvals0 vvals vvals0 :
-  kvals = kvals0 -> vvals = vvals0
-->
-  make_map_vals kvals vvals = make_map_vals kvals0 vvals0.
-Proof.
-  intros. subst. auto.
-Qed.
-
-Fixpoint make_map_vals_inverse (l : list Val) : option (list Val * list Val) :=
-match l with
-| [] => Some ([], [])
-| x::y::xs => match make_map_vals_inverse xs with
-              | Some (vals1, vals2) => Some (x::vals1, y::vals2)
-              | None => None
-              end
-| [x] => None
-end.
-
-Theorem make_map_inverse_length :
-  forall kvals vvals l,
-  make_map_vals_inverse l = Some (kvals, vvals)
-->
-  length l = 2 * length kvals /\ length l = 2 * length vvals.
-Proof.
-  induction kvals; intros.
-  * destruct l; simpl in H.
-    - inversion H. auto.
-    - destruct l.
-      + inversion H.
-      + destruct (make_map_vals_inverse l).
-        ** destruct p. inversion H.
-        ** inversion H.
-  * destruct l; simpl in H.
-    - inversion H.
-    - destruct l.
-      + inversion H.
-      + case_eq (make_map_vals_inverse l); intros; rewrite H0 in H.
-        ** destruct p. inversion H. subst.
-           pose (IHkvals _ _ H0). destruct a0.
-           simpl. lia.
-        ** congruence.
-Qed.
-
-Theorem make_map_inverse_relation :
-  forall kvals vvals v,
-  make_map_vals_inverse v = Some (kvals, vvals)
-->
-  v = make_map_vals kvals vvals.
-Proof.
-  induction kvals; intros.
-  * destruct v; simpl in H.
-    - inversion H. auto.
-    - destruct v0.
-      + inversion H.
-      + destruct (make_map_vals_inverse v1).
-        ** destruct p. inversion H.
-        ** inversion H.
-  * destruct v; simpl in H.
-    - inversion H.
-    - destruct v0.
-      + inversion H.
-      + case_eq (make_map_vals_inverse v1); intros; rewrite H0 in H.
-        ** destruct p. inversion H. subst.
-           pose (IHkvals _ _ H0).
-           simpl. rewrite e. auto.
-        ** congruence.
-Qed.
-
-Theorem make_map_consistent :
-  forall kvals vvals,
-  length kvals = length vvals ->
-  make_map_vals_inverse (make_map_vals kvals vvals) = Some (kvals, vvals).
-Proof.
-  induction kvals; intros.
-  * apply eq_sym, length_zero_iff_nil in H. subst. simpl. auto.
-  * pose (P := element_exist _ _ H). destruct P. destruct H0. subst. inversion H.
-    simpl.
-    pose (P := IHkvals x0 H1). rewrite P. auto.
-Qed.
-
-Theorem map_correcness : forall vals,
-  exists kvals vvals, vals = make_map_vals kvals vvals /\ length kvals = length vvals + length vals mod 2.
-Proof.
-  induction vals using list_length_ind.
-  destruct vals.
-  * exists []. exists []. auto.
-  * destruct vals.
-    - exists [v]. exists []. simpl. auto.
-    - assert (Datatypes.length vals < Datatypes.length (v :: v0 :: vals)). { simpl. lia. }
-      pose (H vals H0). destruct e, H1, H1.
-      exists (v::x). exists (v0::x0).
-      split.
-      + rewrite H1. auto.
-      + simpl length. rewrite <- modulo_2_plus_2.
-        lia.
-Qed.
-
-End map_builders.
